---
title: "Note 6"
author: "Haojie Liu"
date: "2023-10-17"
output: pdf_document
---

### Convolution Methods

$$x_i\sim Ber(p)$$
$$\Sigma x_i \sim Binomial(n,p)$$
$$x_i\sim Geo(p)$$
$$\Sigma x_i \sim NB(n,p,r)$$

$$x_i \sim Possion(\lambda_i)$$
$$\Sigma x_i \sim Possion(\Sigma \lambda_i)$$

$$x \sim X^2_{(1)}$$
$$\Sigma x_i \sim X^2_{(n)}$$

### Composition Methods
$$z\sim N(0,1)$$
$$v=z^2\sim X^2_{(1)}$$
$$V = \Sigma v_i \sim X^2_{(k)}$$
$$\frac{z}{\sqrt{\frac{V}{k}}}\sim t_k$$
$$U\sim X^2_{(n)}$$
$$\frac{\frac{V}{k}}{\frac{U}{n}}\sim F_{k,n}$$

### Transformation of Random Variable


$$x\sim f_X(x)$$
$$y = h(x)\;\;\;c.t.: h(t) \;must\;be\;one-to-one\;function$$
$$x=h^{-1}(y)=g(y)$$

1. $y\sim f_Y(y)$\newline
2. compute $h^{-1}y = g(y)$\newline
3. deliver $x=g(y)$\newline


To find $f_Y(y)$:\newline

scenario 1:\newline


$$F_Y(y)=P(Y\le y) = P(h(x)\le y) = P_X(X\le h^{-1}(y))=P_X(X\le g(y))=F_X(g(y))$$
$$\frac{d}{dy}F_Y(y) = g'(y)f_X(g(y))=f_Y(y)$$

scenario 2:\newline

$$F_Y(y) = P_Y(Y\le y) = P(h(x)\le y) = P(X >h^{-1}(y)) = P_X(X>g(y)) = 1-F_X(g(x))$$
$$\frac{d}{dy}F_Y(y) = -g'(y)f_X(g(y))=f_Y(y)$$

universal:\newline

$$f_Y(y)=|g'(y)|f_X(g(y))$$

**Ex:**
$$x\sim unif(0,1)$$
$$1-x\sim unif(0,1)$$
$$y=h(x) = 1-x\sim unif(0,1)$$
$$h^{-1}(y) = 1-y=g(y)$$
$$f_Y(y)=|-1|f_X(1-y) = 1\sim unif(0,1)$$
**Ex:**

$$X\sim N(0,1)$$
$$f(x) = \frac{1}{\sqrt{2\pi}}e^{-\frac{x^2}{2}}$$
$$y = h(x) = x^2$$
$$x = h^{-1}(y) = \pm\sqrt{y}=g(y)$$
$$f_Y(y) = |\frac{1}{2}y^{-\frac{1}{2}}|\frac{1}{\sqrt{2\pi}}e^{-\frac{y}{2}}$$
For $X^2_{(k)}$, $f(x) = \frac{1}{2^{\frac{k}{2}}\Gamma(\frac{k}{2})}x^{\frac{k}{2}-1}e^{\frac{-x}{2}}$

$$k=1; f(x|k=1) = \frac{1}{\sqrt{2\pi}}x^{-\frac{1}{2}}e^{\frac{-x}{2}}$$

### Mixture Models

$$f_Y(y) = \frac{1}{2}f_+(y) + \frac{1}{2}f_-(y)$$
$$f(y) = \Sigma\theta_if_i(y);\;\Sigma\theta_i =1$$

**Ex:**\newline

$$f_X(x) = \frac{1}{2}f_1(x) + \frac{1}{2}f_2(x)$$
$$f_1(x) = N(0,1)$$
$$f_2(x) = N(3,1)$$
1. Verify if $f(x) \ge 0$\newline
2. $\int^\infty_{-\infty} f(x)dx =1$

**Ex:**
$$f(x) \sim N(0,1)$$
$$f(y) \sim N(0,1)$$
$$f_{XY}(x,y) = f(x)f(y) = \frac{1}{\sqrt{2\pi}}e^{-\frac{x^2+y^2}{2}}$$

$$r = h_1(x,y) = \sqrt{x^2+y^2}$$
$$\theta = h_2(x,y) = tan^{-1}(\frac{y}{x})$$
$$x = h^{-1}(r,\theta) = g(r,\theta) = r\cos(\theta)$$
$$y = g_2(r,\theta)=r\sin(\theta)$$
$$r^2 = x^2+y^2$$
$$\tan(\theta) = \frac{y}{x}$$
$$\cos(\theta) = \frac{x}{r}$$
$$\sin(\theta) = \frac{y}{r}$$

$$f_{R,\theta}(r,\theta) = f_{xy}(g_1(r,\theta), g_2(r,\theta))|J|$$
$$J = \begin{pmatrix}\frac{dg_1(r,\theta)}{dr}&\frac{dg_1(r,\theta)}{d\theta}\\\frac{dg_2(r,\theta)}{dr}&\frac{dg_2(r,\theta)}{d\theta}\end{pmatrix} = \begin{pmatrix}\cos\theta&-r\sin\theta\\\sin\theta&-r\cos\theta\end{pmatrix}$$
$$|J|=r\cos^2\theta+r\sin^2\theta = r$$
$$\frac{1}{\sqrt{2\pi}}e^{-\frac{r^2\cos^2\theta+r^2\sin^2\theta}{2}}r = \frac{1}{\sqrt{2\pi}}e^{-\frac{r^2}{2}}r$$

















